programs/lean/Project/NumInteger/Spec.lean
@@ -746,8 +746,8 @@ theorem func1GlobalHeap_agrees :
 
 theorem func1GlobalHeap_pointsTo [WasmGlobalGS Unit] :
     ([∗map] index ↦ value ∈ func1GlobalHeap,
-      globalPointsTo index value) ⊢
-      globalPointsToAt 0 0 (.i32 1048560) := by
+      globalPointsTo (GF := WasmHeapGF Unit) index value) ⊢
+      globalPointsToAt (GF := WasmHeapGF Unit) 0 0 (.i32 1048560) := by
   unfold func1GlobalHeap
   rw [(BI.BigSepM.bigSepM_insert (get?_empty (⟨0, 0⟩ : GlobalKey))).to_eq,
     BI.BigSepM.bigSepM_empty.to_eq, BI.sep_emp.to_eq]
@@ -3580,8 +3580,8 @@ theorem func0GlobalHeap_agrees :
 
 theorem func0GlobalHeap_pointsTo [WasmGlobalGS Unit] :
     ([∗map] index ↦ value ∈ func0GlobalHeap,
-      globalPointsTo index value) ⊢
-      globalPointsToAt 0 0 (.i32 1048576) := by
+      globalPointsTo (GF := WasmHeapGF Unit) index value) ⊢
+      globalPointsToAt (GF := WasmHeapGF Unit) 0 0 (.i32 1048576) := by
   unfold func0GlobalHeap
   rw [(BI.BigSepM.bigSepM_insert (get?_empty (⟨0, 0⟩ : GlobalKey))).to_eq,
     BI.BigSepM.bigSepM_empty.to_eq, BI.sep_emp.to_eq]
